compiler/scheme/cps/optCpsScript.sml
@@ -44,7 +44,7 @@ Definition opt_cps_def:
   | NONE => EAbs "t" (EVar "t")
   | SOME k => EVar k) /\
   cont_lambda (RCFn e::ks) innerk = EAbs ("m" ++ toString (count_rcarg ks)) (cps_exp e (RCArg (EVar ("m" ++ toString (count_rcarg ks)))::ks) innerk) /\
-  cont_lambda (RCArg e::ks) innerk = EAbs "n" (EApp (EApp (EVar "n") e) (cont_lambda ks innerk))
+  cont_lambda (RCArg e::ks) innerk = EAbs "n" (EApp (EApp e (EVar "n")) (cont_lambda ks innerk))
 Termination
   cheat
 End
@@ -54,8 +54,19 @@ Definition cont_closure_def:
   | NONE => VCl "t" cenv (EVar "t")
   | SOME k => strict_lookup cenv k) /\
   cont_closure (RCFn e::ks) cenv innerk = VCl ("m" ++ toString (count_rcarg ks)) cenv (cps_exp e (RCArg (EVar ("m" ++ toString (count_rcarg ks)))::ks) innerk) /\
-  cont_closure (RCArg e::ks) cenv innerk = VCl "n" cenv (EApp (EApp (EVar "n") e) (cont_lambda ks innerk))
+  cont_closure (RCArg e::ks) cenv innerk = VCl "n" cenv (EApp (EApp e (EVar "n")) (cont_lambda ks innerk))
 End
+
+Theorem cont_lambda_eval:
+  ! eks cenv innerk . ? m . ! ks . cbv_steps m (ks, CExp cenv (cont_lambda eks innerk)) = (ks, CVal (cont_closure eks cenv innerk))
+Proof
+  rpt strip_tac
+  >> Cases_on `eks` >>> HEADGOAL $ Cases_on `innerk`
+  >~ [`ek::eks`] >>> HEADGOAL $ Cases_on `ek`
+  >> simp[opt_cps_def, cont_closure_def]
+  >> qrefine `1`
+  >> simp[cbv_steps, cbv_step_def]
+QED
 
 Definition rich_cbv_continue_def:
   rich_cbv_continue [] env scopes comp tag v = (case scopes of
@@ -136,6 +147,32 @@ End
 Theorem vv_rel_cases = cj 1 vv_env_rel_cases;
 Theorem env_rel_cases = cj 2 vv_env_rel_cases;
 
+Theorem env_rel_sync:
+  ! v cv env cenv x .
+    vv_rel v cv
+    ==>
+    env_rel env cenv ==> env_rel (nsBind x v env) (nsBind ("var" ++ x) cv cenv)
+Proof
+  rpt strip_tac
+  >> gvs[env_rel_cases]
+  >> qx_gen_tac `y`
+  >> Cases_on `x = y`
+  >> gvs[strict_lookup_def]
+QED
+
+Theorem env_rel_sync[allow_rebind] = SRULE [] env_rel_sync;
+
+Theorem env_rel_indifference:
+  ! var env cenv cv .
+    (! x . var <> "var" ++ x)
+    ==>
+    env_rel env cenv ==> env_rel env (nsBind var cv cenv)
+Proof
+  simp[env_rel_cases, strict_lookup_def]
+QED
+
+Theorem env_rel_indifference[allow_rebind, simp] = SRULE [] env_rel_indifference;
+
 Inductive ve_rel:
 [~TVar:]
   vv_rel v (strict_lookup cenv ("var" ++ x))
@@ -147,6 +184,34 @@ Inductive ve_rel:
   ve_rel TAbs (VCl x env e) cenv (EAbs ("var" ++ x) (EAbs "k" (cps_exp e [] (SOME "k"))))
 End
 
+Theorem ve_rel_eval:
+  ! tag v cenv ce .
+    ve_rel tag v cenv ce
+    ==>
+    ? m cv .
+      (! ks . cbv_steps m (ks, CExp cenv ce) = (ks, CVal cv)) /\
+      vv_rel v cv
+Proof
+  rpt strip_tac
+  >> gvs[Once ve_rel_cases]
+  >> qexists `1`
+  >> simp[cbv_steps, cbv_step_def]
+  >> simp[Once vv_rel_cases]
+QED
+
+Theorem ve_rel_indifference:
+  ! var cv tag v cenv ce .
+    (! x . var <> "var" ++ x)
+    ==>
+    ve_rel tag v cenv ce ==> ve_rel tag v (nsBind var cv cenv) ce
+Proof
+  rpt strip_tac
+  >> gvs[Once ve_rel_cases]
+  >> simp[Once ve_rel_cases]
+  >> simp[env_rel_indifference]
+  >> gvs[strict_lookup_def]
+QED
+
 Inductive m_val_rel:
 [~Trivial:]
   ve_rel tag v cenv ce
@@ -157,6 +222,24 @@ Inductive m_val_rel:
   ==>
   m_val_rel Computation v eks cenv (EVar ("m" ++ toString (count_rcarg eks)))
 End
+
+Theorem m_val_rel_eval:
+  ! vtype v eks cenv ce .
+    m_val_rel vtype v eks cenv ce
+    ==>
+    ? m cv .
+      (! ks . cbv_steps m (ks, CExp cenv ce) = (ks, CVal cv)) /\
+      vv_rel v cv
+Proof
+  rpt strip_tac
+  >> gvs[Once m_val_rel_cases] >- (
+    irule ve_rel_eval
+    >> first_assum $ irule_at Any
+  )
+  >> qexists `1`
+  >> simp[cbv_steps, cbv_step_def]
+  >> simp[Once vv_rel_cases]
+QED
 
 Inductive ks_rel:
 [~Id:]
@@ -172,16 +255,53 @@ Inductive ks_rel:
   ks_rel (RCArg (vtype, v)::ks) cenv (RCArg ce::eks)
 End
 
+Theorem ks_rel_indifference:
+  ! var cv ks cenv eks .
+    ks_rel ks cenv eks
+    ==>
+    (! i . i < count_rcarg eks ==> var <> "m" ++ toString i) /\
+    (! x . var <> "var" ++ x)
+    ==>
+    ks_rel ks (nsBind var cv cenv) eks
+Proof
+  gen_tac >> gen_tac
+  >> ho_match_mp_tac ks_rel_ind
+  >> rpt strip_tac
+  >> simp[Once ks_rel_cases]
+  >> gvs[count_rcarg_def]
+  >> gvs[Once m_val_rel_cases]
+  >> simp[Once m_val_rel_cases]
+  >> simp[ve_rel_indifference]
+  >> gvs[strict_lookup_def]
+QED
+
+Theorem ks_rel_indifference[allow_rebind] = SRULE [Once $ GSYM AND_IMP_INTRO] $ SRULE [Once CONJ_COMM, AND_IMP_INTRO] ks_rel_indifference;
+
 Inductive scopes_rel:
 [~NONE:]
   scopes_rel [] kenv NONE
 [~SOME:]
   scopes_rel scopes kenv innerk /\
   ks_rel ks kenv eks /\
+  env_rel env kenv /\
   strict_lookup cenv "k" = cont_closure eks kenv innerk
   ==>
   scopes_rel ((env, ks)::scopes) cenv (SOME "k")
 End
+
+Theorem scopes_rel_indifference:
+  ! var cv scopes cenv innerk .
+    var <> "k"
+    ==>
+    scopes_rel scopes cenv innerk ==> scopes_rel scopes (nsBind var cv cenv) innerk
+Proof
+  rpt strip_tac
+  >> gvs[Once scopes_rel_cases]
+  >> simp[Once scopes_rel_cases]
+  >> gvs[strict_lookup_def]
+  >> irule_at (Pos last) EQ_REFL
+  >> simp[]
+QED
 
 Inductive opt_cps_rel:
 [~RCExp:]
@@ -206,3 +326,226 @@ Inductive opt_cps_rel:
   ==>
   opt_cps_rel ks env scopes (RCVal T tag v) cenv (EApp (EVar "k") ce)
 End
+
+Theorem opt_step_preservation:
+  ! ks ks' env env' scopes scopes' e e' cenv ce .
+    rich_cbv_step (ks, env, scopes, e) = (ks', env', scopes', e') /\
+    opt_cps_rel ks env scopes e cenv ce
+    ==>
+    ? n cenv' ce' .
+      cbv_steps n ([], CExp cenv ce) = ([], CExp cenv' ce') /\
+      opt_cps_rel ks' env' scopes' e' cenv' ce'
+Proof
+  rpt strip_tac
+  >> Cases_on `e`
+  >~ [`RCExp e`] >- (
+    Cases_on `e`
+    >> gvs[rich_cbv_step_def]
+    >> gvs[Once opt_cps_rel_cases]
+    >> simp[opt_cps_def]
+    >> qexists `0`
+    >> simp[cbv_steps]
+    >> simp[Once opt_cps_rel_cases]
+    >> irule_at (Pos hd) EQ_REFL
+    >> simp[Once ve_rel_cases]
+    >> simp[Once ks_rel_cases]
+    >> gvs[Once env_rel_cases]
+  )
+  >~ [`RCVal comp tag v`]
+  >> gvs[rich_cbv_step_def]
+  >> Cases_on `comp` >- (
+    (*Computed term as value*)
+    Cases_on `ks` >- (
+      Cases_on `scopes`
+      >> gvs[rich_cbv_continue_def]
+      >- (
+        gvs[Once opt_cps_rel_cases]
+        >> gvs[Once ks_rel_cases]
+        >> gvs[Once scopes_rel_cases]
+        >> qexists `0`
+        >> simp[cbv_steps]
+        >> simp[Once opt_cps_rel_cases]
+        >> simp[Once ks_rel_cases]
+        >> simp[Once scopes_rel_cases]
+        >> irule_at (Pos last) EQ_REFL
+        >> simp[]
+      )
+      >~ [`scope::scopes'`]
+      >> PairCases_on `scope`
+      >> gvs[Once opt_cps_rel_cases]
+      >> gvs[Once ks_rel_cases]
+      >> gvs[Once scopes_rel_cases]
+      >> gvs[cont_closure_def]
+      >> qexists `0`
+      >> simp[cbv_steps]
+      >> simp[Once opt_cps_rel_cases]
+      >> irule_at (Pos last) EQ_REFL
+      >> simp[]
+    )
+    >~ [`k::ks'`]
+    >> Cases_on `k`
+    >~ [`RCFn e`] >- (
+      gvs[rich_cbv_continue_def]
+      >> gvs[Once opt_cps_rel_cases]
+      >> gvs[Once ks_rel_cases]
+      >> gvs[cont_closure_def]
+      >> qrefine `n+3`
+      >> simp[cbv_steps, cbv_step_def, cbv_continue_def]
+      >> drule_then assume_tac ve_rel_eval
+      >> gvs[]
+      >> qrefine `n+m`
+      >> simp[cbv_steps_ADD]
+      >> qrefine `n+1`
+      >> simp[cbv_steps, cbv_step_def, cbv_continue_def]
+      >> qexists `0`
+      >> simp[cbv_steps]
+      >> simp[Once opt_cps_rel_cases]
+      >> irule_at (Pos hd) EQ_REFL
+      >> simp[Once ks_rel_cases]
+      >> simp[m_val_rel_cases]
+      >> simp[strict_lookup_def]
+      >> simp[scopes_rel_indifference]
+      >> simp[ks_rel_indifference]
+    )
+    >~ [`RCArg tv`]
+    >> PairCases_on `tv`
+    >> Cases_on `tv1`
+    >~ [`VCl x env e`]
+    >> gvs[rich_cbv_continue_def]
+    >> gvs[Once opt_cps_rel_cases]
+    >> gvs[Once ks_rel_cases]
+    >> gvs[cont_closure_def]
+    >> qrefine `n+3`
+    >> simp[cbv_steps, cbv_step_def, cbv_continue_def]
+    >> drule_then assume_tac ve_rel_eval
+    >> gvs[]
+    >> qrefine `n+m`
+    >> simp[cbv_steps_ADD]
+    >> qrefine `n+3`
+    >> simp[cbv_steps, cbv_step_def, cbv_continue_def]
+    >> gvs[Once m_val_rel_cases]
+    >>> HEADGOAL (
+      qspecl_then [`"n"`, `cv`] (assume_tac o SRULE []) ve_rel_indifference
+      >> pop_assum $ rev_drule_then assume_tac
+      >> drule_then assume_tac ve_rel_eval
+      >> gvs[]
+      >> qrefine `n+m'`
+      >> simp[cbv_steps_ADD]
+      >> qpat_x_assum `! _. cbv_steps _ _ = _` kall_tac
+    )
+    >>> LASTGOAL (
+      qrefine `n+1`
+      >> simp[cbv_steps, cbv_step_def]
+      >> gvs[strict_lookup_def]
+    )
+    >> gvs[vv_rel_cases]
+    >> qrefine `n+5`
+    >> simp[cbv_steps, cbv_step_def, cbv_continue_def, strict_lookup_def]
+    >> qmatch_goalsub_abbrev_tac `cbv_steps _ (_, CExp newenv _)`
+    >> qspecl_then [`eks'`, `newenv`, `innerk`] assume_tac cont_lambda_eval
+    >> gvs[]
+    >> unabbrev_all_tac
+    >> qrefine `n+m'`
+    >> simp[cbv_steps_ADD]
+    >> qrefine `n+1`
+    >> simp[cbv_steps, cbv_step_def, cbv_continue_def]
+    >> qexists `0`
+    >> simp[cbv_steps]
+    >> simp[Once opt_cps_rel_cases]
+    >> irule_at (Pos hd) EQ_REFL
+    >> simp[Once ks_rel_cases]
+    >> simp[Once scopes_rel_cases]
+    >> simp[strict_lookup_def]
+    >> irule_at (Pos last) EQ_REFL
+    >> irule_at (Pos hd) env_rel_indifference
+    >> simp[]
+    >> irule_at (Pos hd) env_rel_sync
+    >> simp[vv_rel_cases]
+    >> simp[scopes_rel_indifference]
+    >> simp[ks_rel_indifference]
+  )
+  (*Trivial term as value*)
+  >> Cases_on `ks` >- (
+    Cases_on `scopes`
+    >> gvs[rich_cbv_continue_def]
+    >- (
+      gvs[Once opt_cps_rel_cases]
+      >> gvs[Once ks_rel_cases]
+      >> gvs[Once scopes_rel_cases]
+      >> qexists `0`
+      >> simp[cbv_steps]
+      >> simp[Once opt_cps_rel_cases]
+      >> simp[Once ks_rel_cases]
+      >> simp[Once scopes_rel_cases]
+      >> irule_at (Pos hd) EQ_REFL
+      >> simp[]
+    )
+    >~ [`scope::scopes'`]
+    >> PairCases_on `scope`
+    >> gvs[Once opt_cps_rel_cases]
+    >> gvs[Once ks_rel_cases]
+    >> gvs[Once scopes_rel_cases]
+    >> gvs[cont_closure_def]
+    >> qexists `0`
+    >> simp[cbv_steps]
+    >> simp[Once opt_cps_rel_cases]
+    >> irule_at (Pos last) EQ_REFL
+    >> simp[opt_cps_def]
+  )
+  >~ [`k::ks'`]
+  >> Cases_on `k`
+  >~ [`RCFn e`] >- (
+    gvs[rich_cbv_continue_def]
+    >> gvs[Once opt_cps_rel_cases]
+    >> gvs[Once ks_rel_cases]
+    >> qexists `0`
+    >> simp[cbv_steps]
+    >> simp[Once opt_cps_rel_cases]
+    >> simp[opt_cps_def]
+    >> irule_at (Pos hd) EQ_REFL
+    >> simp[Once ks_rel_cases]
+    >> simp[m_val_rel_cases]
+  )
+  >~ [`RCArg tv`]
+  >> PairCases_on `tv`
+  >> Cases_on `tv1`
+  >~ [`VCl x env e`]
+  >> gvs[rich_cbv_continue_def]
+  >> gvs[Once opt_cps_rel_cases]
+  >> gvs[Once ks_rel_cases]
+  >> simp[opt_cps_def]
+  >> qrefine `n+2`
+  >> simp[cbv_steps, cbv_step_def]
+  >> drule_then assume_tac m_val_rel_eval
+  >> gvs[]
+  >> qrefine `n+m`
+  >> simp[cbv_steps_ADD]
+  >> qrefine `n+1`
+  >> simp[cbv_steps, cbv_step_def, cbv_continue_def]
+  >> gvs[Once vv_rel_cases]
+  >> drule_then assume_tac ve_rel_eval
+  >> gvs[]
+  >> gvs[Once m_val_rel_cases]
+  >> qrefine `n+m'`
+  >> simp[cbv_steps_ADD]
+  >> qrefine `n+1`
+  >> simp[cbv_steps, cbv_step_def, cbv_continue_def]
+  >> qrefine `n+2`
+  >> simp[cbv_steps, cbv_step_def, cbv_continue_def]
+  >> qspecl_then [`eks'`, `cenv`, `innerk`] assume_tac cont_lambda_eval
+  >> gvs[]
+  >> qrefine `n+m''`
+  >> simp[cbv_steps_ADD]
+  >> qrefine `n+1`
+  >> simp[cbv_steps, cbv_step_def, cbv_continue_def]
+  >> qexists `0`
+  >> simp[cbv_steps]
+  >> simp[Once opt_cps_rel_cases]
+  >> irule_at (Pos hd) EQ_REFL
+  >> simp[Once ks_rel_cases]
+  >> simp[Once scopes_rel_cases]
+  >> simp[strict_lookup_def]
+  >> irule_at (Pos last) EQ_REFL
+  >> irule_at (Pos hd) env_rel_indifference
+  >> simp[env_rel_sync]
+QED
